theories/Concurrent.v
@@ -1,0 +1,835 @@
+From Stdlib Require Import MSets.
+From PackageCalculus Require Import Prelude Core.
+
+Create HintDb cmp_conc.
+Create Rewrite HintDb cmp_conc.
+
+Module Concurrent (N V : UsualOrderedType) (G : UsualOrderedType).
+  Module C := Core N V.
+  Module Pkg := C.Pkg.
+  Module PkgSet := C.PkgSet.
+  Module VSet := C.VSet.
+
+  Module ParentElt := PairUOT Pkg Pkg.
+  Module ParentRel := FSetUOT ParentElt.
+
+  Record IsResolution
+      (R : PkgSet.t) (D : C.DepRel.t) (g : V.t -> G.t) (r : Pkg.t)
+      (S : PkgSet.t) (pi : ParentRel.t) : Prop :=
+    { res_subset : PkgSet.Subset S R
+    ; res_root_mem : PkgSet.In r S
+    ; res_parent_closure :
+        forall p, PkgSet.In p S ->
+        forall (n : N.t) (vs : VSet.t),
+          C.DepRel.In (p, (n, vs)) D ->
+          exists! v, VSet.In v vs /\
+            PkgSet.In (n, v) S /\ ParentRel.In ((n, v), p) pi
+    ; res_version_granularity :
+        forall (n : N.t) (v v' : V.t),
+          PkgSet.In (n, v) S -> PkgSet.In (n, v') S -> v <> v' -> g v <> g v'
+    ; res_parent_subset :
+        forall c p, ParentRel.In (c, p) pi -> PkgSet.In c S /\ PkgSet.In p S }.
+
+  Module Reduction.
+    Definition IsSplit (g : V.t -> G.t) (vs : VSet.t) : Prop :=
+      exists u1 u2, VSet.In u1 vs /\ VSet.In u2 vs /\ g u1 <> g u2.
+
+    Definition IsDirect (g : V.t -> G.t) (vs : VSet.t) : Prop :=
+      forall u1 u2, VSet.In u1 vs -> VSet.In u2 vs -> g u1 = g u2.
+
+    Module GEqb := UOTEqb G.
+    (* kept as an alias: "same granule" is what the guards below mean *)
+    Definition granEqb : G.t -> G.t -> bool := GEqb.eqb.
+
+    Lemma granEqb_iff : forall a b, granEqb a b = true <-> a = b.
+    Proof. exact GEqb.eqb_true_iff. Qed.
+
+    Definition isSplitb (g : V.t -> G.t) (vs : VSet.t) : bool :=
+      VSet.exists_ (fun u1 =>
+        VSet.exists_ (fun u2 => negb (granEqb (g u1) (g u2))) vs) vs.
+
+    Definition isDirectb (g : V.t -> G.t) (vs : VSet.t) : bool :=
+      VSet.for_all (fun u1 =>
+        VSet.for_all (fun u2 => granEqb (g u1) (g u2)) vs) vs.
+
+    Lemma isSplitb_iff : forall g vs, isSplitb g vs = true <-> IsSplit g vs.
+    Proof.
+      intros g vs; unfold isSplitb, IsSplit.
+      rewrite VSet.exists_spec'.
+      split.
+      - intros [u1 [Hu1 H1]].
+        rewrite VSet.exists_spec' in H1.
+        destruct H1 as [u2 [Hu2 H2]].
+        exists u1, u2; repeat split; try assumption.
+        apply Bool.negb_true_iff in H2.
+        intro E; rewrite <- granEqb_iff in E; congruence.
+      - intros [u1 [u2 [Hu1 [Hu2 Hne]]]].
+        exists u1; split; [exact Hu1 |].
+        rewrite VSet.exists_spec'.
+        exists u2; split; [exact Hu2 |].
+        apply Bool.negb_true_iff, Bool.not_true_iff_false.
+        intro E; exact (Hne (proj1 (granEqb_iff _ _) E)).
+    Qed.
+
+    Lemma isSplitb_false_iff : forall g vs,
+        isSplitb g vs = false <-> IsDirect g vs.
+    Proof.
+      intros g vs; split.
+      - intros H u1 u2 Hu1 Hu2.
+        destruct (G.eq_dec (g u1) (g u2)) as [E | NE]; [exact E |].
+        assert (isSplitb g vs = true) as Ht
+          by (apply isSplitb_iff; exists u1, u2; auto).
+        congruence.
+      - intro H; destruct (isSplitb g vs) eqn:E; [| reflexivity].
+        apply isSplitb_iff in E; destruct E as [u1 [u2 [Hu1 [Hu2 Hne]]]].
+        contradiction (Hne (H u1 u2 Hu1 Hu2)).
+    Qed.
+
+    Lemma isDirectb_iff : forall g vs, isDirectb g vs = true <-> IsDirect g vs.
+    Proof.
+      intros g vs; unfold isDirectb, IsDirect.
+      rewrite VSet.for_all_spec'.
+      split.
+      - intros H u1 u2 Hu1 Hu2.
+        specialize (H u1 Hu1).
+        rewrite VSet.for_all_spec' in H.
+        exact (proj1 (granEqb_iff _ _) (H u2 Hu2)).
+      - intros H u1 Hu1.
+        rewrite VSet.for_all_spec'.
+        intros u2 Hu2; apply granEqb_iff; apply H; assumption.
+    Qed.
+
+    Module NG := PairUOT N G.
+    Module NVN := TripleUOT N V N.
+    Module NGF := UOTCompareFacts NG.
+    Module NVNF := UOTCompareFacts NVN.
+    #[local] Hint Rewrite NGF.compare_eq_iff NVNF.compare_eq_iff : cmp_conc.
+    #[local] Hint Extern 1 => cmp_by NGF.compare_antisym : cmp_conc.
+    #[local] Hint Extern 1 => cmp_by NVNF.compare_antisym : cmp_conc.
+    #[local] Hint Extern 1 => cmp_by NGF.compare_lt_trans : cmp_conc.
+    #[local] Hint Extern 1 => cmp_by NVNF.compare_lt_trans : cmp_conc.
+
+    Module Name.
+      Inductive name : Type :=
+      | Granular (n : N.t) (w : G.t)
+      | Intermediate (n : N.t) (v : V.t) (m : N.t).
+      Definition t := name.
+
+      Definition compare (x y : t) : comparison :=
+        match x, y with
+        | Granular n1 w1, Granular n2 w2 => NG.compare (n1, w1) (n2, w2)
+        | Granular _ _, Intermediate _ _ _ => Lt
+        | Intermediate _ _ _, Granular _ _ => Gt
+        | Intermediate n1 v1 m1, Intermediate n2 v2 m2 =>
+            NVN.compare (n1, (v1, m1)) (n2, (v2, m2))
+        end.
+
+      Lemma compare_eq_iff : forall x y, compare x y = Eq <-> x = y.
+      Proof. cmp_eq_iff cmp_conc. Qed.
+
+      Lemma compare_antisym : forall x y, compare y x = CompOpp (compare x y).
+      Proof. cmp_antisym cmp_conc. Qed.
+
+      Lemma compare_lt_trans : forall x y z,
+          compare x y = Lt -> compare y z = Lt -> compare x z = Lt.
+      Proof. cmp_lt_trans cmp_conc. Qed.
+    End Name.
+
+    Module GF := UOTCompareFacts G.
+    Module VF := UOTCompareFacts V.
+    #[local] Hint Rewrite GF.compare_eq_iff VF.compare_eq_iff : cmp_conc.
+    #[local] Hint Extern 1 => cmp_by GF.compare_antisym : cmp_conc.
+    #[local] Hint Extern 1 => cmp_by VF.compare_antisym : cmp_conc.
+    #[local] Hint Extern 1 => cmp_by GF.compare_lt_trans : cmp_conc.
+    #[local] Hint Extern 1 => cmp_by VF.compare_lt_trans : cmp_conc.
+
+    Module Version.
+      Inductive version : Type :=
+      | Orig (v : V.t)
+      | Gran (w : G.t).
+      Definition t := version.
+
+      Definition compare (x y : t) : comparison :=
+        match x, y with
+        | Orig v1, Orig v2 => V.compare v1 v2
+        | Orig _, Gran _ => Lt
+        | Gran _, Orig _ => Gt
+        | Gran w1, Gran w2 => G.compare w1 w2
+        end.
+
+      Lemma compare_eq_iff : forall x y, compare x y = Eq <-> x = y.
+      Proof. cmp_eq_iff cmp_conc. Qed.
+
+      Lemma compare_antisym : forall x y, compare y x = CompOpp (compare x y).
+      Proof. cmp_antisym cmp_conc. Qed.
+
+      Lemma compare_lt_trans : forall x y z,
+          compare x y = Lt -> compare y z = Lt -> compare x z = Lt.
+      Proof. cmp_lt_trans cmp_conc. Qed.
+    End Version.
+
+    Module NameOT := UOTFromCompare Name.
+    Module VersionOT := UOTFromCompare Version.
+    Module T := Core NameOT VersionOT.
+
+    Definition embedPkg (g : V.t -> G.t) (p : Pkg.t) : T.Pkg.t :=
+      (Name.Granular (fst p) (g (snd p)), Version.Orig (snd p)).
+
+    Module SOptp := SetOps Pkg T.Pkg PkgSet T.PkgSet.
+    Definition embedSet (g : V.t -> G.t) (R : PkgSet.t) : T.PkgSet.t :=
+      SOptp.map (embedPkg g) R.
+
+    Module SOvcv := SetOps V VersionOT VSet T.VSet.
+    Definition embedVS (vs : VSet.t) : T.VSet.t :=
+      SOvcv.map Version.Orig vs.
+
+    Definition gransOfVS (g : V.t -> G.t) (vs : VSet.t) : T.VSet.t :=
+      SOvcv.map (fun u => Version.Gran (g u)) vs.
+
+    Definition filterGran (g : V.t -> G.t) (u : V.t) (vs : VSet.t) : VSet.t :=
+      VSet.filter (fun w => granEqb (g w) (g u)) vs.
+
+    Module SOvtp := SetOps V T.Pkg VSet T.PkgSet.
+    Module SOdtp := SetOps C.DepElt T.Pkg C.DepRel T.PkgSet.
+    Definition reduceReal (R : PkgSet.t) (D : C.DepRel.t) (g : V.t -> G.t) :
+        T.PkgSet.t :=
+      T.PkgSet.union (embedSet g R)
+        (SOdtp.unionMap (fun '((n, v), (m, vs)) =>
+             if isSplitb g vs
+             then SOvtp.map (fun u =>
+                      (Name.Intermediate n v m, Version.Gran (g u)))
+                    vs
+             else T.PkgSet.empty)
+           D).
+
+    Module SOvtd := SetOps V T.DepElt VSet T.DepRel.
+    Module SOdtd := SetOps C.DepElt T.DepElt C.DepRel T.DepRel.
+    Definition reduceDepsDirect (D : C.DepRel.t) (g : V.t -> G.t) :
+        T.DepRel.t :=
+      SOdtd.unionMap (fun '((n, v), (m, vs)) =>
+          if isDirectb g vs
+          then SOvtd.map (fun u =>
+                   ((Name.Granular n (g v), Version.Orig v),
+                    (Name.Granular m (g u), embedVS vs)))
+                 vs
+          else T.DepRel.empty)
+        D.
+
+    Definition reduceDepsSplitEntry (D : C.DepRel.t) (g : V.t -> G.t) :
+        T.DepRel.t :=
+      SOdtd.filterMap (fun '((n, v), (m, vs)) =>
+          if isSplitb g vs
+          then Some ((Name.Granular n (g v), Version.Orig v),
+                     (Name.Intermediate n v m, gransOfVS g vs))
+          else None)
+        D.
+
+    Definition reduceDepsSplitFanout (D : C.DepRel.t) (g : V.t -> G.t) :
+        T.DepRel.t :=
+      SOdtd.unionMap (fun '((n, v), (m, vs)) =>
+          if isSplitb g vs
+          then SOvtd.map (fun u =>
+                   ((Name.Intermediate n v m, Version.Gran (g u)),
+                    (Name.Granular m (g u), embedVS (filterGran g u vs))))
+                 vs
+          else T.DepRel.empty)
+        D.
+
+    Definition reduceDepsEmpty (D : C.DepRel.t) (g : V.t -> G.t) : T.DepRel.t :=
+      SOdtd.filterMap (fun '((n, v), (m, vs)) =>
+          if VSet.is_empty vs
+          then Some ((Name.Granular n (g v), Version.Orig v),
+                     (Name.Intermediate n v m, T.VSet.empty))
+          else None)
+        D.
+
+    Definition reduceDeps (D : C.DepRel.t) (g : V.t -> G.t) : T.DepRel.t :=
+      T.DepRel.union (reduceDepsDirect D g)
+        (T.DepRel.union (reduceDepsSplitEntry D g)
+           (T.DepRel.union (reduceDepsSplitFanout D g) (reduceDepsEmpty D g))).
+
+    Lemma mem_filterGran : forall g u0 vs u,
+        VSet.In u (filterGran g u0 vs) <-> VSet.In u vs /\ g u = g u0.
+    Proof.
+      intros g u0 vs u; unfold filterGran.
+      rewrite VSet.filter_spec'.
+      rewrite granEqb_iff; reflexivity.
+    Qed.
+
+    Lemma mem_reduceReal : forall R D g q,
+        T.PkgSet.In q (reduceReal R D g) <->
+        (exists p, PkgSet.In p R /\ q = embedPkg g p) \/
+        (exists n v m vs u,
+            C.DepRel.In ((n, v), (m, vs)) D /\ IsSplit g vs /\ VSet.In u vs /\
+            q = (Name.Intermediate n v m, Version.Gran (g u))).
+    Proof.
+      intros R D g q; unfold reduceReal, embedSet.
+      rewrite T.PkgSet.union_spec, SOptp.mem_map, SOdtp.mem_unionMap.
+      apply or_iff_compat_l; split.
+      - intros [[[n v] [m vs]] [HeD Hh]]; cbn beta iota in Hh.
+        destruct (isSplitb g vs) eqn:Hs; [| destruct (SOdtp.empty_in _ Hh)].
+        apply SOvtp.mem_map in Hh; destruct Hh as [u [Hu ->]].
+        exists n, v, m, vs, u; repeat split; try assumption.
+        apply isSplitb_iff; exact Hs.
+      - intros [n [v [m [vs [u [HD [Hspl [Hu ->]]]]]]]].
+        exists ((n, v), (m, vs)); split; [exact HD | cbn beta iota].
+        apply isSplitb_iff in Hspl; rewrite Hspl.
+        apply SOvtp.mem_map; exists u; split; [exact Hu | reflexivity].
+    Qed.
+
+    Lemma mem_reduceDepsDirect : forall D g y,
+        T.DepRel.In y (reduceDepsDirect D g) <->
+        exists n v m vs u,
+          C.DepRel.In ((n, v), (m, vs)) D /\ IsDirect g vs /\ VSet.In u vs /\
+          y = ((Name.Granular n (g v), Version.Orig v),
+               (Name.Granular m (g u), embedVS vs)).
+    Proof.
+      intros D g y; unfold reduceDepsDirect; rewrite SOdtd.mem_unionMap.
+      split.
+      - intros [[[n v] [m vs]] [HeD Hh]]; cbn beta iota in Hh.
+        destruct (isDirectb g vs) eqn:Hd; [| destruct (SOdtd.empty_in _ Hh)].
+        apply SOvtd.mem_map in Hh; destruct Hh as [u [Hu ->]].
+        exists n, v, m, vs, u; repeat split; try assumption.
+        apply isDirectb_iff; exact Hd.
+      - intros [n [v [m [vs [u [HD [Hdir [Hu ->]]]]]]]].
+        exists ((n, v), (m, vs)); split; [exact HD | cbn beta iota].
+        apply isDirectb_iff in Hdir; rewrite Hdir.
+        apply SOvtd.mem_map; exists u; split; [exact Hu | reflexivity].
+    Qed.
+
+    Lemma mem_reduceDepsSplitEntry : forall D g y,
+        T.DepRel.In y (reduceDepsSplitEntry D g) <->
+        exists n v m vs,
+          C.DepRel.In ((n, v), (m, vs)) D /\ IsSplit g vs /\
+          y = ((Name.Granular n (g v), Version.Orig v),
+               (Name.Intermediate n v m, gransOfVS g vs)).
+    Proof.
+      intros D g y; unfold reduceDepsSplitEntry; rewrite SOdtd.mem_filterMap.
+      split.
+      - intros [[[n v] [m vs]] [HeD Hh]]; cbn beta iota in Hh.
+        destruct (isSplitb g vs) eqn:Hs; [| discriminate].
+        injection Hh as <-.
+        exists n, v, m, vs; repeat split; try assumption.
+        apply isSplitb_iff; exact Hs.
+      - intros [n [v [m [vs [HD [Hspl ->]]]]]].
+        exists ((n, v), (m, vs)); split; [exact HD | cbn beta iota].
+        apply isSplitb_iff in Hspl; rewrite Hspl; reflexivity.
+    Qed.
+
+    Lemma mem_reduceDepsSplitFanout : forall D g y,
+        T.DepRel.In y (reduceDepsSplitFanout D g) <->
+        exists n v m vs u,
+          C.DepRel.In ((n, v), (m, vs)) D /\ IsSplit g vs /\ VSet.In u vs /\
+          y = ((Name.Intermediate n v m, Version.Gran (g u)),
+               (Name.Granular m (g u), embedVS (filterGran g u vs))).
+    Proof.
+      intros D g y; unfold reduceDepsSplitFanout; rewrite SOdtd.mem_unionMap.
+      split.
+      - intros [[[n v] [m vs]] [HeD Hh]]; cbn beta iota in Hh.
+        destruct (isSplitb g vs) eqn:Hs; [| destruct (SOdtd.empty_in _ Hh)].
+        apply SOvtd.mem_map in Hh; destruct Hh as [u [Hu ->]].
+        exists n, v, m, vs, u; repeat split; try assumption.
+        apply isSplitb_iff; exact Hs.
+      - intros [n [v [m [vs [u [HD [Hspl [Hu ->]]]]]]]].
+        exists ((n, v), (m, vs)); split; [exact HD | cbn beta iota].
+        apply isSplitb_iff in Hspl; rewrite Hspl.
+        apply SOvtd.mem_map; exists u; split; [exact Hu | reflexivity].
+    Qed.
+
+    Lemma mem_reduceDepsEmpty : forall D g y,
+        T.DepRel.In y (reduceDepsEmpty D g) <->
+        exists n v m,
+          C.DepRel.In ((n, v), (m, VSet.empty)) D /\
+          y = ((Name.Granular n (g v), Version.Orig v),
+               (Name.Intermediate n v m, T.VSet.empty)).
+    Proof.
+      intros D g y; unfold reduceDepsEmpty; rewrite SOdtd.mem_filterMap.
+      split.
+      - intros [[[n v] [m vs]] [HeD Hh]]; cbn beta iota in Hh.
+        destruct (VSet.is_empty vs) eqn:He; [| discriminate].
+        injection Hh as <-.
+        apply VSet.is_empty_iff in He; subst vs.
+        exists n, v, m; split; [assumption | reflexivity].
+      - intros [n [v [m [HD ->]]]].
+        exists ((n, v), (m, VSet.empty)); split; [exact HD | simpl];
+          reflexivity.
+    Qed.
+
+    Lemma mem_reduceDeps : forall D g y,
+        T.DepRel.In y (reduceDeps D g) <->
+        (exists n v m vs u,
+            C.DepRel.In ((n, v), (m, vs)) D /\ IsDirect g vs /\ VSet.In u vs /\
+            y = ((Name.Granular n (g v), Version.Orig v),
+                 (Name.Granular m (g u), embedVS vs))) \/
+        ((exists n v m vs,
+             C.DepRel.In ((n, v), (m, vs)) D /\ IsSplit g vs /\
+             y = ((Name.Granular n (g v), Version.Orig v),
+                  (Name.Intermediate n v m, gransOfVS g vs))) \/
+         ((exists n v m vs u,
+              C.DepRel.In ((n, v), (m, vs)) D /\ IsSplit g vs /\ VSet.In u vs /\
+              y = ((Name.Intermediate n v m, Version.Gran (g u)),
+                   (Name.Granular m (g u), embedVS (filterGran g u vs)))) \/
+          (exists n v m,
+              C.DepRel.In ((n, v), (m, VSet.empty)) D /\
+              y = ((Name.Granular n (g v), Version.Orig v),
+                   (Name.Intermediate n v m, T.VSet.empty))))).
+    Proof.
+      intros D g y; unfold reduceDeps.
+      rewrite !T.DepRel.union_spec.
+      rewrite mem_reduceDepsDirect, mem_reduceDepsSplitEntry,
+        mem_reduceDepsSplitFanout, mem_reduceDepsEmpty.
+      reflexivity.
+    Qed.
+
+    Definition tryInvPkg (g : V.t -> G.t) (p' : T.Pkg.t) : option Pkg.t :=
+      match p' with
+      | (Name.Granular n w, Version.Orig v) =>
+          if G.eq_dec w (g v) then Some (n, v) else None
+      | _ => None
+      end.
+
+    Lemma tryInvPkg_embed : forall g p, tryInvPkg g (embedPkg g p) = Some p.
+    Proof.
+      intros g [n v]; unfold tryInvPkg, embedPkg; cbn [fst snd].
+      destruct (G.eq_dec (g v) (g v)) as [_ | NE];
+        [reflexivity | contradiction NE; reflexivity].
+    Qed.
+
+    Lemma tryInvPkg_some : forall g (p' : T.Pkg.t) (p : Pkg.t),
+        tryInvPkg g p' = Some p -> embedPkg g p = p'.
+    Proof.
+      intros g [[n w | n v m] [v' | w']] p H; cbn [tryInvPkg] in H;
+        try discriminate.
+      destruct (G.eq_dec w (g v')) as [-> | NE]; [| discriminate].
+      injection H as <-; reflexivity.
+    Qed.
+
+    Module SOtpp := SetOps T.Pkg Pkg T.PkgSet PkgSet.
+    Lemma embedPkg_injective : forall g (p q : Pkg.t),
+        embedPkg g p = embedPkg g q -> p = q.
+    Proof.
+      intro g;
+        exact (SOtpp.emb_injective (tryInvPkg g) (embedPkg g)
+                 (tryInvPkg_embed g)).
+    Qed.
+
+    Definition concurrentResolution (g : V.t -> G.t) (S : T.PkgSet.t)
+        : PkgSet.t :=
+      SOtpp.filterMap (tryInvPkg g) S.
+
+    Lemma mem_concurrentResolution : forall g (S : T.PkgSet.t) (p : Pkg.t),
+        PkgSet.In p (concurrentResolution g S) <-> T.PkgSet.In (embedPkg g p) S.
+    Proof.
+      intro g; unfold concurrentResolution.
+      exact (SOtpp.mem_filterMap_inv (tryInvPkg g) (embedPkg g)
+               (tryInvPkg_embed g) (tryInvPkg_some g)).
+    Qed.
+
+    Definition piGuardb (g : V.t -> G.t) (S : T.PkgSet.t)
+        (n : N.t) (v : V.t) (m : N.t) (vs : VSet.t) (u : V.t) : bool :=
+      andb (T.PkgSet.mem (Name.Granular m (g u), Version.Orig u) S)
+        (andb (T.PkgSet.mem (Name.Granular n (g v), Version.Orig v) S)
+           (implb (isSplitb g vs)
+              (VSet.exists_ (fun u0 =>
+                   andb (T.PkgSet.mem
+                           (Name.Intermediate n v m, Version.Gran (g u0)) S)
+                     (granEqb (g u) (g u0)))
+                 vs))).
+
+    Lemma piGuardb_iff : forall g S n v m vs u,
+        piGuardb g S n v m vs u = true <->
+        T.PkgSet.In (Name.Granular m (g u), Version.Orig u) S /\
+        T.PkgSet.In (Name.Granular n (g v), Version.Orig v) S /\
+        (IsSplit g vs ->
+           exists u0, VSet.In u0 vs /\
+             T.PkgSet.In (Name.Intermediate n v m, Version.Gran (g u0)) S /\
+             g u = g u0).
+    Proof.
+      intros g S n v m vs u; unfold piGuardb.
+      rewrite !Bool.andb_true_iff, Bool.implb_true_iff, !T.PkgSet.mem_spec,
+        isSplitb_iff.
+      rewrite VSet.exists_spec'.
+      split.
+      - intros [H1 [H2 H3]]; repeat split; try assumption.
+        intro Hs; destruct (H3 Hs) as [u0 [Hu0 Hb]].
+        apply Bool.andb_true_iff in Hb; destruct Hb as [Hm Hg].
+        apply T.PkgSet.mem_spec in Hm.
+        exists u0; repeat split; try assumption.
+        exact (proj1 (granEqb_iff _ _) Hg).
+      - intros [H1 [H2 H3]]; repeat split; try assumption.
+        intro Hs; destruct (H3 Hs) as [u0 [Hu0 [Hm Hg]]].
+        exists u0; split; [exact Hu0 |].
+        apply Bool.andb_true_iff; split.
+        + apply T.PkgSet.mem_spec; exact Hm.
+        + apply granEqb_iff; exact Hg.
+    Qed.
+
+    Module SOvpp := SetOps V ParentElt VSet ParentRel.
+    Module SOdpp := SetOps C.DepElt ParentElt C.DepRel ParentRel.
+    Definition parents (D : C.DepRel.t) (g : V.t -> G.t) (S : T.PkgSet.t) :
+        ParentRel.t :=
+      SOdpp.unionMap (fun '((n, v), (m, vs)) =>
+          SOvpp.filterMap (fun u =>
+              if piGuardb g S n v m vs u then Some ((m, u), (n, v)) else None)
+            vs)
+        D.
+
+    Lemma mem_parents : forall D g S (pair : ParentElt.t),
+        ParentRel.In pair (parents D g S) <->
+        exists n v m vs u,
+          C.DepRel.In ((n, v), (m, vs)) D /\
+          T.PkgSet.In (Name.Granular n (g v), Version.Orig v) S /\
+          VSet.In u vs /\
+          T.PkgSet.In (Name.Granular m (g u), Version.Orig u) S /\
+          (IsSplit g vs ->
+             exists u0, VSet.In u0 vs /\
+               T.PkgSet.In (Name.Intermediate n v m, Version.Gran (g u0)) S /\
+               g u = g u0) /\
+          pair = ((m, u), (n, v)).
+    Proof.
+      intros D g S pair; unfold parents; rewrite SOdpp.mem_unionMap.
+      split.
+      - intros [[[n v] [m vs]] [HeD Hh]]; cbn beta iota in Hh.
+        apply SOvpp.mem_filterMap in Hh; destruct Hh as [u [Hu Hc]];
+          cbn beta iota in Hc.
+        destruct (piGuardb g S n v m vs u) eqn:Hg; [| discriminate].
+        injection Hc as <-.
+        apply piGuardb_iff in Hg; destruct Hg as [H1 [H2 H3]].
+        exists n, v, m, vs, u; repeat split; assumption.
+      - intros [n [v [m [vs [u [HD [HvS [Hu [HuS [Hsc ->]]]]]]]]]].
+        exists ((n, v), (m, vs)); split; [exact HD | cbn beta iota].
+        apply SOvpp.mem_filterMap; exists u; split; [exact Hu | cbn beta iota].
+        assert (Hg : piGuardb g S n v m vs u = true)
+          by (apply piGuardb_iff; repeat split; assumption).
+        rewrite Hg; reflexivity.
+    Qed.
+
+    Lemma embedPkg_mem_reduceReal : forall g (p : Pkg.t) R D,
+        T.PkgSet.In (embedPkg g p) (reduceReal R D g) -> PkgSet.In p R.
+    Proof.
+      intros g p R D H; apply mem_reduceReal in H.
+      destruct H as [[q [HqR Hq]] | [n [v [m [vs [u [_ [_ [_ Hq]]]]]]]]].
+      - apply embedPkg_injective in Hq; subst q; exact HqR.
+      - destruct p as [pn pv]; unfold embedPkg in Hq; simpl in Hq.
+        injection Hq as Hq _; discriminate.
+    Qed.
+
+    Lemma mem_reduceDeps_direct : forall D g n v m vs u0,
+        C.DepRel.In ((n, v), (m, vs)) D -> IsDirect g vs -> VSet.In u0 vs ->
+        T.DepRel.In ((Name.Granular n (g v), Version.Orig v),
+                     (Name.Granular m (g u0), embedVS vs))
+          (reduceDeps D g).
+    Proof.
+      intros; apply mem_reduceDeps.
+      left; exists n, v, m, vs, u0; repeat split; assumption.
+    Qed.
+
+    Lemma mem_reduceDeps_split1 : forall D g n v m vs,
+        C.DepRel.In ((n, v), (m, vs)) D -> IsSplit g vs ->
+        T.DepRel.In ((Name.Granular n (g v), Version.Orig v),
+                     (Name.Intermediate n v m, gransOfVS g vs))
+          (reduceDeps D g).
+    Proof.
+      intros; apply mem_reduceDeps.
+      right; left; exists n, v, m, vs; repeat split; assumption.
+    Qed.
+
+    Lemma mem_reduceDeps_split2 : forall D g n v m vs u0,
+        C.DepRel.In ((n, v), (m, vs)) D -> IsSplit g vs -> VSet.In u0 vs ->
+        T.DepRel.In ((Name.Intermediate n v m, Version.Gran (g u0)),
+                     (Name.Granular m (g u0), embedVS (filterGran g u0 vs)))
+          (reduceDeps D g).
+    Proof.
+      intros; apply mem_reduceDeps.
+      right; right; left; exists n, v, m, vs, u0; repeat split; assumption.
+    Qed.
+
+    Lemma mem_reduceDeps_empty : forall D g n v m,
+        C.DepRel.In ((n, v), (m, VSet.empty)) D ->
+        T.DepRel.In ((Name.Granular n (g v), Version.Orig v),
+                     (Name.Intermediate n v m, T.VSet.empty))
+          (reduceDeps D g).
+    Proof.
+      intros; apply mem_reduceDeps.
+      right; right; right; exists n, v, m; split; [assumption | reflexivity].
+    Qed.
+
+    Theorem concurrent_soundness :
+      forall (R : PkgSet.t) (D : C.DepRel.t) (g : V.t -> G.t) (r : Pkg.t)
+             (S : T.PkgSet.t),
+        C.FunctionalInName D ->
+        T.IsResolution (reduceReal R D g) (reduceDeps D g) (embedPkg g r) S ->
+        IsResolution R D g r (concurrentResolution g S) (parents D g S).
+    Proof.
+      intros R D g r S Hfunc Hres.
+      destruct Hres as [Hsub Hroot Hdep Huniq].
+      constructor.
+      - intros p Hp; apply mem_concurrentResolution in Hp.
+        exact (embedPkg_mem_reduceReal g p R D (Hsub _ Hp)).
+      - apply mem_concurrentResolution; exact Hroot.
+      - intros [pn pv] Hp m vs Hdep0.
+        apply mem_concurrentResolution in Hp;
+          unfold embedPkg in Hp; simpl in Hp.
+        destruct (VSet.is_empty vs) eqn:Hemp.
+        + apply VSet.is_empty_iff in Hemp; subst vs.
+          destruct (Hdep _ Hp _ _ (mem_reduceDeps_empty D g pn pv m Hdep0))
+            as [cv [Hcv _]].
+          destruct (SOvcv.empty_in _ Hcv).
+        + destruct (isSplitb g vs) eqn:Hs.
+          * apply isSplitb_iff in Hs.
+            destruct (Hdep _ Hp _ _
+                (mem_reduceDeps_split1 D g pn pv m vs Hdep0 Hs))
+              as [cv0 [Hcv0 Hcv0S]].
+            unfold gransOfVS in Hcv0; apply SOvcv.mem_map in Hcv0;
+              destruct Hcv0 as [u0 [Hu0 ->]].
+            destruct (Hdep _ Hcv0S _ _
+                (mem_reduceDeps_split2 D g pn pv m vs u0 Hdep0 Hs Hu0))
+              as [cv [Hcv HcvS]].
+            unfold embedVS in Hcv; apply SOvcv.mem_map in Hcv;
+              destruct Hcv as [u [Hu ->]].
+            apply mem_filterGran in Hu; destruct Hu as [Hu Hgu].
+            assert (T.PkgSet.In (Name.Granular m (g u), Version.Orig u) S)
+              as HuS
+              by (rewrite Hgu; exact HcvS).
+            exists u; split.
+            { split; [exact Hu | split].
+              - apply mem_concurrentResolution; exact HuS.
+              - apply mem_parents.
+                exists pn, pv, m, vs, u.
+                repeat split; try assumption.
+                intros _; exists u0; repeat split; assumption. }
+            { intros u' [Hu' [Hu'S Hpi']].
+              apply mem_concurrentResolution in Hu'S; unfold embedPkg in Hu'S;
+                simpl in Hu'S.
+              apply mem_parents in Hpi'.
+              destruct Hpi'
+                as [n' [v' [m' [vs' [u'' [Hdep' [_ [_ [_ [Hsc Heq]]]]]]]]]].
+              injection Heq as <- <- <- <-.
+              assert (vs' = vs) as -> by (exact (Hfunc _ _ _ _ Hdep' Hdep0)).
+              destruct (Hsc Hs) as [u0' [Hu0' [Hu0'S Hgu']]].
+              assert (Version.Gran (g u0') = Version.Gran (g u0)) as Hg0
+                by (exact (Huniq _ _ _ Hu0'S Hcv0S)).
+              injection Hg0 as Hg0.
+              rewrite Hg0 in Hgu'; rewrite Hgu' in Hu'S.
+              assert (T.PkgSet.In (Name.Granular m (g u0), Version.Orig u) S)
+                as HuS0
+                by (rewrite <- Hgu; exact HuS).
+              pose proof (Huniq _ _ _ Hu'S HuS0) as He.
+              injection He as He; congruence. }
+          * pose proof (proj1 (isSplitb_false_iff g vs) Hs) as Hdir.
+            destruct (VSet.choose vs) as [u0 |] eqn:Hch.
+            2:{ apply VSet.choose_spec2 in Hch.
+                rewrite <- VSet.is_empty_spec in Hch; congruence. }
+            pose proof (VSet.choose_spec1 Hch) as Hu0.
+            destruct (Hdep _ Hp _ _
+                (mem_reduceDeps_direct D g pn pv m vs u0 Hdep0 Hdir Hu0))
+              as [cv [Hcv HcvS]].
+            unfold embedVS in Hcv; apply SOvcv.mem_map in Hcv;
+              destruct Hcv as [u [Hu ->]].
+            pose proof (Hdir u u0 Hu Hu0) as Hgu.
+            assert (T.PkgSet.In (Name.Granular m (g u), Version.Orig u) S)
+              as HuS
+              by (rewrite Hgu; exact HcvS).
+            exists u; split.
+            { split; [exact Hu | split].
+              - apply mem_concurrentResolution; exact HuS.
+              - apply mem_parents.
+                exists pn, pv, m, vs, u.
+                repeat split; try assumption.
+                intro Hsplit; exfalso.
+                destruct Hsplit as [u1 [u2 [Hu1 [Hu2 Hne]]]].
+                exact (Hne (Hdir u1 u2 Hu1 Hu2)). }
+            { intros u' [Hu' [Hu'S _]].
+              apply mem_concurrentResolution in Hu'S; unfold embedPkg in Hu'S;
+                simpl in Hu'S.
+              pose proof (Hdir u' u0 Hu' Hu0) as Hgu'.
+              rewrite Hgu' in Hu'S.
+              pose proof (Huniq _ _ _ Hu'S HcvS) as He.
+              injection He as He; congruence. }
+      - intros n v v' Hv Hv' Hne Hg.
+        apply mem_concurrentResolution in Hv, Hv'; unfold embedPkg in Hv, Hv';
+          simpl in Hv, Hv'.
+        rewrite Hg in Hv.
+        pose proof (Huniq _ _ _ Hv Hv') as He.
+        injection He as He; exact (Hne He).
+      - intros c p Hcp.
+        apply mem_parents in Hcp.
+        destruct Hcp as [n [v [m [vs [u [_ [HvS [_ [HuS [_ Heq]]]]]]]]]].
+        injection Heq as -> ->.
+        split; apply mem_concurrentResolution; [exact HuS | exact HvS].
+    Qed.
+
+    Definition coreResolution (S : PkgSet.t) (pi : ParentRel.t)
+        (D : C.DepRel.t) (g : V.t -> G.t) : T.PkgSet.t :=
+      T.PkgSet.union (SOptp.map (embedPkg g) S)
+        (SOdtp.unionMap (fun '((n, v), (m, vs)) =>
+             if andb (isSplitb g vs) (PkgSet.mem (n, v) S)
+             then SOvtp.filterMap (fun u =>
+                      if andb (PkgSet.mem (m, u) S)
+                           (ParentRel.mem ((m, u), (n, v)) pi)
+                      then Some (Name.Intermediate n v m, Version.Gran (g u))
+                      else None)
+                    vs
+             else T.PkgSet.empty)
+           D).
+
+    Lemma mem_coreResolution : forall S pi D g (q : T.Pkg.t),
+        T.PkgSet.In q (coreResolution S pi D g) <->
+        (exists n v, PkgSet.In (n, v) S /\
+           q = (Name.Granular n (g v), Version.Orig v)) \/
+        (exists n v m vs u,
+           C.DepRel.In ((n, v), (m, vs)) D /\ PkgSet.In (n, v) S /\
+           IsSplit g vs /\ PkgSet.In (m, u) S /\ VSet.In u vs /\
+           ParentRel.In ((m, u), (n, v)) pi /\
+           q = (Name.Intermediate n v m, Version.Gran (g u))).
+    Proof.
+      intros S pi D g q; unfold coreResolution.
+      rewrite T.PkgSet.union_spec, SOptp.mem_map, SOdtp.mem_unionMap.
+      assert (Hfst :
+        (exists p, PkgSet.In p S /\ q = embedPkg g p) <->
+        (exists n v, PkgSet.In (n, v) S /\
+           q = (Name.Granular n (g v), Version.Orig v))).
+      { split.
+        - intros [[n v] [HpS ->]];
+            exists n, v; split; [exact HpS | reflexivity].
+        - intros [n [v [HnS ->]]]; exists (n, v); auto. }
+      rewrite Hfst; apply or_iff_compat_l.
+      split.
+      - intros [[[n v] [m vs]] [HeD Hh]]; cbn beta iota in Hh.
+        destruct (andb (isSplitb g vs) (PkgSet.mem (n, v) S)) eqn:Hg;
+          [| destruct (SOdtp.empty_in _ Hh)].
+        apply Bool.andb_true_iff in Hg; destruct Hg as [Hs Hnv].
+        apply isSplitb_iff in Hs; apply PkgSet.mem_spec in Hnv.
+        apply SOvtp.mem_filterMap in Hh; destruct Hh as [u [Hu Hc]];
+          cbn beta iota in Hc.
+        destruct (andb (PkgSet.mem (m, u) S)
+                    (ParentRel.mem ((m, u), (n, v)) pi)) eqn:Hb;
+          [| discriminate].
+        injection Hc as <-.
+        apply Bool.andb_true_iff in Hb; destruct Hb as [Hmu Hpi].
+        apply PkgSet.mem_spec in Hmu; apply ParentRel.mem_spec in Hpi.
+        exists n, v, m, vs, u; repeat split; assumption.
+      - intros [n [v [m [vs [u [HD [Hnv [Hs [Hmu [Hu [Hpi ->]]]]]]]]]]].
+        exists ((n, v), (m, vs)); split; [exact HD | cbn beta iota].
+        assert (andb (isSplitb g vs) (PkgSet.mem (n, v) S) = true) as ->.
+        { apply Bool.andb_true_iff; split;
+            [apply isSplitb_iff; exact Hs | apply PkgSet.mem_spec; exact Hnv]. }
+        apply SOvtp.mem_filterMap; exists u; split; [exact Hu | cbn beta iota].
+        assert (andb (PkgSet.mem (m, u) S)
+                  (ParentRel.mem ((m, u), (n, v)) pi) = true) as ->.
+        { apply Bool.andb_true_iff; split;
+            [apply PkgSet.mem_spec; exact Hmu
+            | apply ParentRel.mem_spec; exact Hpi]. }
+        reflexivity.
+    Qed.
+
+    Lemma mem_coreResolution_granular : forall S pi D g n v,
+        PkgSet.In (n, v) S ->
+        T.PkgSet.In (Name.Granular n (g v), Version.Orig v)
+          (coreResolution S pi D g).
+    Proof.
+      intros; apply mem_coreResolution.
+      left; exists n, v; split; [assumption | reflexivity].
+    Qed.
+
+    Lemma mem_coreResolution_intermediate : forall S pi D g n v m vs u,
+        C.DepRel.In ((n, v), (m, vs)) D -> PkgSet.In (n, v) S ->
+        IsSplit g vs -> PkgSet.In (m, u) S -> VSet.In u vs ->
+        ParentRel.In ((m, u), (n, v)) pi ->
+        T.PkgSet.In (Name.Intermediate n v m, Version.Gran (g u))
+          (coreResolution S pi D g).
+    Proof.
+      intros; apply mem_coreResolution.
+      right; exists n, v, m, vs, u; repeat split; assumption.
+    Qed.
+
+    Theorem concurrent_completeness :
+      forall (R : PkgSet.t) (D : C.DepRel.t) (g : V.t -> G.t) (r : Pkg.t)
+             (S : PkgSet.t) (pi : ParentRel.t),
+        C.FunctionalInName D ->
+        IsResolution R D g r S pi ->
+        T.IsResolution (reduceReal R D g) (reduceDeps D g)
+          (embedPkg g r) (coreResolution S pi D g).
+    Proof.
+      intros R D g r S pi Hfunc Hres.
+      destruct Hres as [Hsub Hroot Hpc Hvg Hps].
+      constructor.
+      - intros q Hq; apply mem_coreResolution in Hq.
+        apply mem_reduceReal.
+        destruct Hq as
+          [[n [v [Hnv ->]]]
+          | [n [v [m [vs [u [HD [Hnv [Hs [Hmu [Hu [Hpi ->]]]]]]]]]]]].
+        + left; exists (n, v); split; [apply Hsub; exact Hnv | reflexivity].
+        + right; exists n, v, m, vs, u; repeat split; try assumption.
+      - destruct r as [rn rv].
+        exact (mem_coreResolution_granular S pi D g rn rv Hroot).
+      - intros q Hq md vsd Hd.
+        apply mem_coreResolution in Hq.
+        apply mem_reduceDeps in Hd.
+        destruct Hq as
+          [[n [v [Hnv ->]]]
+          | [n [v [m [vs [u [HD [Hnv [Hs [Hmu [Hu [Hpi ->]]]]]]]]]]]].
+        + destruct Hd as [Hd | [Hd | [Hd | Hd]]].
+          * destruct Hd as [n' [v' [m' [vs' [u' [HD' [Hdir' [Hu' Heq]]]]]]]].
+            injection Heq as <- Hgv <- -> ->.
+            destruct (Hpc _ Hnv _ _ HD') as [u [[Huv [HmuS Hpiu]] _]].
+            exists (Version.Orig u); split.
+            { unfold embedVS; apply SOvcv.mem_map;
+                exists u; split; [exact Huv | reflexivity]. }
+            { rewrite <- (Hdir' u u' Huv Hu').
+              exact (mem_coreResolution_granular S pi D g m' u HmuS). }
+          * destruct Hd as [n' [v' [m' [vs' [HD' [Hs' Heq]]]]]].
+            injection Heq as <- Hgv <- -> ->.
+            destruct (Hpc _ Hnv _ _ HD') as [u [[Huv [HmuS Hpiu]] _]].
+            exists (Version.Gran (g u)); split.
+            { unfold gransOfVS; apply SOvcv.mem_map;
+                exists u; split; [exact Huv | reflexivity]. }
+            { exact (mem_coreResolution_intermediate S pi D g n v m' vs' u
+                       HD' Hnv Hs' HmuS Huv Hpiu). }
+          * destruct Hd as [n' [v' [m' [vs' [u' [HD' [Hs' [Hu' Heq]]]]]]]].
+            discriminate Heq.
+          * destruct Hd as [n' [v' [m' [HD' Heq]]]].
+            injection Heq as <- Hgv <- -> ->.
+            destruct (Hpc _ Hnv _ _ HD') as [u [[Huv _] _]].
+            destruct (VSet.empty_spec Huv).
+        + destruct Hd as [Hd | [Hd | [Hd | Hd]]].
+          * destruct Hd as [n' [v' [m' [vs' [u' [HD' [Hdir' [Hu' Heq]]]]]]]].
+            discriminate Heq.
+          * destruct Hd as [n' [v' [m' [vs' [HD' [Hs' Heq]]]]]].
+            discriminate Heq.
+          * destruct Hd as [n' [v' [m' [vs' [u'' [HD' [Hs' [Hu'' Heq]]]]]]]].
+            injection Heq as <- <- <- Hgu -> ->.
+            assert (vs' = vs) as -> by (exact (Hfunc _ _ _ _ HD' HD)).
+            exists (Version.Orig u); split.
+            { unfold embedVS; apply SOvcv.mem_map; exists u; split;
+                [| reflexivity].
+              apply mem_filterGran; split; [exact Hu | exact Hgu]. }
+            { rewrite <- Hgu.
+              exact (mem_coreResolution_granular S pi D g m u Hmu). }
+          * destruct Hd as [n' [v' [m' [HD' Heq]]]].
+            discriminate Heq.
+      - intros nm cv1 cv2 H1 H2.
+        apply mem_coreResolution in H1, H2.
+        destruct H1 as
+          [[n1 [v1 [Hm1 He1]]]
+          | [n1 [v1 [m1 [vs1 [u1
+              [Hd1 [Hnv1 [Hs1 [Hmu1 [Hu1 [Hpi1 He1]]]]]]]]]]]];
+        destruct H2 as
+          [[n2 [v2 [Hm2 He2]]]
+          | [n2 [v2 [m2 [vs2 [u2
+              [Hd2 [Hnv2 [Hs2 [Hmu2 [Hu2 [Hpi2 He2]]]]]]]]]]]].
+        + injection He1 as -> ->; injection He2 as <- Hg ->.
+          destruct (V.eq_dec v1 v2) as [-> | NE]; [reflexivity |].
+          exfalso; exact (Hvg n1 v1 v2 Hm1 Hm2 NE Hg).
+        + injection He1 as -> ->; discriminate He2.
+        + injection He1 as -> ->; discriminate He2.
+        + injection He1 as -> ->; injection He2 as <- <- <- ->.
+          assert (vs2 = vs1) as -> by (exact (Hfunc _ _ _ _ Hd2 Hd1)).
+          destruct (Hpc _ Hnv1 _ _ Hd1) as [w [_ Huniq]].
+          pose proof (Huniq u1 (conj Hu1 (conj Hmu1 Hpi1))) as E1.
+          pose proof (Huniq u2 (conj Hu2 (conj Hmu2 Hpi2))) as E2.
+          congruence.
+    Qed.
+  End Reduction.
+
+End Concurrent.
